src/goose_lang/fmcounter.v
@@ -1,18 +1,18 @@
 (** Crash instances for fmcounter. *)
 From iris.proofmode Require Import base tactics classes.
-From Perennial.algebra Require Export fmcounter.
+From iris.base_logic.lib Require Import mnat.
 From Perennial.goose_lang Require Import crash_modality lifting.
 
 Section instances.
 Context `{ffi_semantics: ext_semantics}.
 Context `{!ffi_interp ffi}.
-Context `{!fmcounterG Σ, !heapG Σ}.
+Context `{!mnatG Σ, !heapG Σ}.
 
-Global Instance fmcounter_lb_durable γ n:
-  IntoCrash (fmcounter_lb γ n) (λ _, fmcounter_lb γ n).
+Global Instance mnat_own_lb_durable γ n:
+  IntoCrash (mnat_own_lb γ n) (λ _, mnat_own_lb γ n).
 Proof. rewrite /IntoCrash. iApply post_crash_nodep. Qed.
 
-Global Instance fmcounter_durable γ q n:
-  IntoCrash (fmcounter γ q n) (λ _, fmcounter γ q n).
+Global Instance mnat_own_auth_durable γ q n:
+  IntoCrash (mnat_own_auth γ q n) (λ _, mnat_own_auth γ q n).
 Proof. rewrite /IntoCrash. iApply post_crash_nodep. Qed.
 End instances.
