src/program_proof/wal/invariant.v
@@ -28,6 +28,8 @@ Class walG Σ :=
     wal_stable_mapG  :> mapG Σ nat unit;
     wal_logger_pos   :> ghost_varG Σ u64;
     wal_base_disk    :> inG Σ (agreeR (leibnizO disk));
+    (* TODO: switch over to Iris mnat entirely *)
+    wal_fmcounter    :> fmcounterG Σ;
   }.
 
 Section goose_lang.
